unity/models/reschedule.lean
@@ -1,0 +1,80 @@
+
+import unity.models.nondet
+import unity.refinement
+
+namespace nondet
+
+open predicate
+open unity
+
+universe variable u
+
+variables {lbl α : Type}
+
+structure evt_ref (mc : @prog α lbl) (ea ec : @event α) : Prop :=
+  (sim : ⟦ ec.step_of ⟧ ⟹ ⟦ ea.step_of ⟧)
+  (delay : ea.coarse_sch ↦ ec.coarse_sch in mc)
+  (stable : unless mc ec.coarse_sch (~ea.coarse_sch))
+  (resched : ea.fine_sch ↦ ec.fine_sch in mc)
+
+structure refined (m₀ m₁ : @prog α lbl) : Prop :=
+  (sim_init : m₁^.first ⟹ m₀^.first)
+  (sim : ⟦ is_step m₁ ⟧ ⟹ ⟦ is_step m₀ ⟧)
+  (delay : ∀ e, m₀^.coarse_sch_of e ↦ m₁^.coarse_sch_of e in m₁)
+  (stable : ∀ e, unless m₁ (m₁^.coarse_sch_of e) (~m₀^.coarse_sch_of e))
+  (resched : ∀ e, m₀^.fine_sch_of e ↦ m₁^.fine_sch_of e in m₁)
+
+lemma event_refinement {m₀ m₁ : @prog α lbl}
+   (INIT : m₁^.first ⟹ m₀^.first)
+   (EVT : ∀ e, evt_ref m₁ (m₀.event' e) (m₁.event' e))
+: refined m₀ m₁ :=
+begin
+  apply refined.mk,
+  { apply INIT },
+  { simp [is_step_exists_event],
+    apply p_or_entails_p_or_right,
+    apply p_exists_entails_p_exists, intro e,
+    apply (EVT e).sim },
+  all_goals
+    { intro e, cases e with e,
+      try { apply True_leads_to_True },
+      try { simp, apply True_unless } },
+  { apply (EVT e).delay },
+  { apply (EVT e).stable },
+  { apply (EVT e).resched },
+end
+
+variables  (m₀ m₁ : @prog α lbl)
+
+open temporal
+
+theorem soundness : refined m₀ m₁ → unity.refinement.refined m₀ m₁ :=
+sorry
+-- begin
+--   intros R τ M₁,
+--   apply nondet.prog.ex.mk,
+--   { apply R.sim_init,
+--     apply M₁.init },
+--   { intro i,
+--     apply R.sim,
+--     unfold temporal.action is_step nondet.is_step,
+--     cases M₁.safety i with ev H,
+--     existsi ev,
+--     unfold nondet.prog.step_of,
+--     rw R.sim _ ,
+--     apply H },
+--   { intros e COARSE₀ FINE₀,
+--     assert COARSE₁ : (<>[]•prog.coarse_sch_of m₁ e) τ,
+--     { clear FINE₀,
+--       note UNLESS := unless_sem _ τ (R.stable e),
+--       note COARSE₀ := inf_often_of_stable _ COARSE₀,
+--       note COARSE₀' := inf_often_of_leads_to (system_sem.leads_to_sem (R.delay e) _ M₁) COARSE₀, },
+--     assert FINE₁ : ([]<>•prog.fine_sch_of m₁ e) τ,
+--     {  },
+--     apply hence_map _ _ (M₁.liveness _ COARSE₁ FINE₁),
+--     apply ex_map,
+--     rw R.sim,
+--     intro, apply id },
+-- end
+
+end nondet
