unity/refinement.lean
@@ -1,0 +1,21 @@
+
+import unity.logic
+import unity.predicate
+import unity.temporal
+
+namespace unity.refinement
+
+open unity
+open temporal
+open predicate
+
+universe variables u
+
+variables {α : Type u}
+
+def refined (s s' : α) [system_sem α] : Prop :=
+system_sem.ex s' ⟹ system_sem.ex s
+
+infix ` ⊑ `:80 := refined
+
+end unity.refinement
